Add DGK encryption and zero check impls

code/experimental/he/Hacl.Impl.HE.DGK.fst
@@ -60,8 +60,8 @@ type proper_secret_raw
         let h = as_snat hp h in
         (p > 1 /\ q > 1 /\ isprm p /\ isprm q /\ p <> q /\ n = p * q /\
 
-         u > 1 /\ divides u (p-1) /\ divides u (q-1) /\
-         v > 1 /\ divides v (p-1) /\ divides v (q-1) /\
+         u > 1 /\ u < n /\ divides u (p-1) /\ divides u (q-1) /\
+         v > 1 /\ v < n /\ divides v (p-1) /\ divides v (q-1) /\
 
          g < n /\ isunit #(p*q) g /\ mult_order #(p*q) g = u * v /\
 
@@ -92,6 +92,7 @@ type secret_mem h (#nLen:bn_len_s) (s:secret nLen) =
                   loc (Sec?.v s);
                   loc (Sec?.g s);
                   loc (Sec?.h s)]
+
 
 val as_spec_sk:
      #nLen:bn_len_s
@@ -127,7 +128,8 @@ type proper_public_raw
         let u = as_snat hp u in
         let g = as_snat hp g in
         let h = as_snat hp h in
-        (u > 1 /\ g < n /\ h < n /\ isunit #n g /\ isunit #n h))
+
+        (u > 1 /\ u < n /\ g < n /\ h < n /\ isunit #n g /\ isunit #n h))
 
 type proper_public h (#nLen:bn_len_s) (p:public nLen) =
   proper_public_raw h
@@ -151,11 +153,11 @@ val as_spec_pk:
   -> hp:mem
   -> p:public nLen{public_mem hp p /\ proper_public hp p}
   -> GTot (p':S.public)
-let as_spec_pk #nLen hp s =
-  S.Public (as_snat hp (Pub?.n s))
-           (as_snat hp (Pub?.u s))
-           (as_snat hp (Pub?.g s))
-           (as_snat hp (Pub?.h s))
+let as_spec_pk #nLen hp p =
+  S.Public (as_snat hp (Pub?.n p))
+           (as_snat hp (Pub?.u p))
+           (as_snat hp (Pub?.g p))
+           (as_snat hp (Pub?.h p))
 
 val s2p: #nLen:bn_len_s -> s:secret nLen ->
   Stack (public nLen)
@@ -166,3 +168,82 @@ val s2p: #nLen:bn_len_s -> s:secret nLen ->
          public_mem h1 p /\
          as_spec_pk h1 p = S.s2p (as_spec_sk h0 s))
 let s2p #nLen s = Pub (Sec?.n s) (Sec?.u s) (Sec?.g s) (Sec?.h s)
+
+#reset-options "--z3rlimit 200 --max_fuel 0 --max_ifuel 0"
+
+val encrypt:
+     #nLen:bn_len_s
+  -> pk:public nLen
+  -> r:lbignum nLen
+  -> m:lbignum nLen
+  -> res:lbignum nLen
+  -> Stack unit
+     (requires fun h ->
+      proper_public h pk /\ public_mem h pk /\
+      as_snat h r > 1 /\
+      as_snat h m < as_snat h (Pub?.u pk) /\
+      live h r /\ live h m /\ live h res /\
+      disjoint m (Pub?.g pk) /\
+      disjoint (Pub?.h pk) r /\
+      disjoint (Pub?.n pk) res)
+     (ensures fun h0 _ h1 ->
+      modifies1 res h0 h1 /\
+      as_snat h1 res = S.encrypt (as_spec_pk h0 pk) (as_snat h0 r) (as_snat h0 m)
+      )
+let encrypt #nLen pk r m res =
+  bn_len_s_fits nLen;
+
+  push_frame ();
+  let hp0 = FStar.HyperStack.ST.get () in
+
+  let tmp1 = create nLen (u64 0) in
+  let tmp2 = create nLen (u64 0) in
+
+  let n = Pub?.n pk in
+  let g = Pub?.g pk in
+  let h = Pub?.h pk in
+
+  bn_modular_exp n g m tmp1;
+  bn_modular_exp n h r tmp2;
+  bn_modular_mul n tmp1 tmp2 res;
+
+  let hp = FStar.HyperStack.ST.get () in
+  to_fe_idemp #(as_snat hp0 n) (as_snat hp0 g);
+  to_fe_idemp #(as_snat hp0 n) (as_snat hp0 h);
+  assert (as_snat hp res =
+          ( *% ) #(as_snat hp0 n)
+          (fexp #(as_snat hp0 n) (as_snat hp0 g) (as_snat hp0 m))
+          (fexp #(as_snat hp0 n) (as_snat hp0 h) (as_snat hp0 r))
+         );
+
+  pop_frame ()
+
+val check_is_zero:
+     #nLen:bn_len_s
+  -> sk:secret nLen
+  -> c:lbignum nLen
+  -> Stack bool
+     (requires fun h ->
+      proper_secret h sk /\ secret_mem h sk /\
+      as_snat h c < as_snat h (Sec?.u sk) /\
+      live h c /\
+      disjoint (Sec?.v sk) c)
+     (ensures fun h0 b h1 ->
+      modifies0 h0 h1 /\
+      b = S.check_is_zero (as_spec_sk h0 sk) (as_snat h0 c)
+      )
+let check_is_zero #nLen sk c =
+  bn_len_s_fits nLen;
+  push_frame ();
+  let hp0 = FStar.HyperStack.ST.get () in
+
+  let tmp = create nLen (u64 0) in
+  to_fe_idemp #(as_snat hp0 (Sec?.n sk)) (as_snat hp0 c);
+  bn_modular_exp (Sec?.n sk) c (Sec?.v sk) tmp;
+
+  let one:lbignum 1ul = bn_one #1ul in
+
+  let b = bn_is_equal tmp one in
+
+  pop_frame ();
+  b
